\documentclass{article}

\usepackage[margin=0.5in]{geometry}
\usepackage{amsmath}
\usepackage{mathtools}

\begin{document}

\begin{equation}
	c_x = x_1 - x_c
\end{equation}

\begin{equation}
	c_y = y_1 - y_c
\end{equation}

\begin{equation}
	c = \begin{bmatrix}
	c_x\\
	c_y
	\end{bmatrix}
\end{equation}

\begin{equation}
	D(q) = jacobian(c) = \frac{\partial c}{\partial q}
\end{equation}

\begin{equation}
	\dot{c} = \frac{\partial c}{\partial q} \dot{q} = D(q)\dot{q}
\end{equation}

\begin{equation}
	\ddot{c} = \frac{d}{dt}(D(q)\dot{q}) = D(q)\ddot{q} +  \frac{\partial }{\partial q}(D(q)\dot{q})\dot{q} = 0
\end{equation}

\begin{equation}
	d = \frac{\partial }{\partial q}(D(q)\dot{q})\dot{q}
\end{equation}

\begin{equation}
	e = D(q)*(M(q)\backslash(D(q)^\top *(\alpha*c + \beta*\dot{c})))
\end{equation}

\begin{equation}
	\begin{bmatrix}
	M(q)_{4x4} & -D(q)^\top_{4x2}\\
	D(q)_{2x4} & 0_{2x2}
	\end{bmatrix}
	\begin{bmatrix}
	\ddot{q}_{4x1}\\
	\lambda_{2x1}
	\end{bmatrix} = 
	\begin{bmatrix}
	(- C(q, \dot{q}) - G(q))_{4x1}\\
	-(d + e)_{2x1}
	\end{bmatrix}
\end{equation}



\end{document}